

Part 1

$$\begin{aligned}
 1. (a) \quad & \frac{d}{dx} [(3x^2 - 7x + 1)^5 (4x - 3)^3] \\
 &= (3x^2 - 7x + 1)^5 \frac{d}{dx} (4x - 3)^3 + (4x - 3)^3 \frac{d}{dx} (3x^2 - 7x + 1)^5 \\
 &= (3x^2 - 7x + 1)^5 [3(4x - 3)^2] (4) + (4x - 3)^3 [5(3x^2 - 7x + 1)^4 (6x - 7)] \\
 &= (4x - 3)^2 (3x^2 - 7x + 1)^4 [12(3x^2 - 7x + 1) + 5(4x - 3)(6x - 7)] \\
 &= (4x - 3)^2 (3x^2 - 7x + 1)^4 (36x^2 - 84x + 12 + 120x^2 - 230x + 105) \\
 &= (4x - 3)^2 (3x^2 - 7x + 1)^4 (156x^2 - 314x + 117)
 \end{aligned}$$

$$\begin{aligned}
 (b) \quad & \frac{d}{dx} \left[ \frac{4x^2 - 1}{(2x + 7)^3} \right] \\
 &= \frac{(2x + 7)^3 \frac{d}{dx} (4x^2 - 1) - (4x^2 - 1) \frac{d}{dx} (2x + 7)^3}{(2x + 7)^6} \\
 &= \frac{(2x + 7)^3 (8x) - (4x^2 - 1) [3(2x + 7)^2 (2)]}{(2x + 7)^6} \\
 &= \frac{(2x + 7)(8x) - (4x^2 - 1)(6)}{(2x + 7)^6} \\
 &= \frac{16x^2 + 56x - 24x^2 + 6}{(2x + 7)^6} \\
 &= \frac{-8x^2 + 56x + 6}{(2x + 7)^6}
 \end{aligned}$$

$$\begin{aligned}
 (c) \quad & \frac{d}{dx} \sin^2(1 - 3x) \\
 &= [2 \sin(1 - 3x)] [\cos(1 - 3x)] \frac{d}{dx} (1 - 3x) \\
 &= -6 \sin(1 - 3x) \cos(1 - 3x) \\
 &= -6 \left( \frac{1}{2} \right) [\sin(2 - 6x)] \\
 &= -3 \sin(2 - 6x)
 \end{aligned}$$

$$\begin{aligned}
 (d) \quad & \frac{d}{dx} \sqrt{\cos 2x} \\
 &= \frac{1}{2\sqrt{\cos 2x}} \left( \frac{d}{dx} \cos 2x \right) \\
 &= \frac{-2 \sin 2x}{2\sqrt{\cos 2x}} \\
 &= -\frac{\sin 2x}{\sqrt{\cos 2x}}
 \end{aligned}$$

$$\begin{aligned}
 (e) \quad & \frac{d}{dx} \tan(\cos^{-1} x) \\
 &= [\sec^2(\cos^{-1} x)] \left( -\frac{1}{\sqrt{1 - x^2}} \right) \\
 &= \frac{1}{\cos^2(\cos^{-1} x)} \left( -\frac{1}{\sqrt{1 - x^2}} \right) \\
 &= -\frac{1}{x^2 \sqrt{1 - x^2}}
 \end{aligned}$$

## Part 1 (cont.)

1. (f)  $\frac{d}{dx} \sin^{-1}(x^2)$

(cont.)

$$= \frac{1}{\sqrt{1-x^4}} \left( \frac{d}{dx} x^2 \right)$$

$$= \frac{2x}{\sqrt{1-x^4}}$$

(g)  $\frac{d}{dx} \tan(e^{3x})$

$$= \frac{1}{1+e^{6x}} \left( \frac{d}{dx} e^{3x} \right)$$

$$= \frac{3e^{3x}}{1+e^{6x}}$$

(h)  $\frac{d}{dx} \ln \left( \frac{e^{x^2+7x} \sin 3x}{\sqrt{x}} \right)$

$$= \frac{d}{dx} (\ln e^{x^2+7x} + \ln \sin 3x - \ln \sqrt{x})$$

$$= \frac{d}{dx} (x^2+7x + \ln \sin 3x - \ln \sqrt{x})$$

$$= 2x+7 + \frac{3 \cos 3x}{\sin 3x} - \left( \frac{1}{\sqrt{x}} \right) \left( \frac{1}{2\sqrt{x}} \right)$$

$$= 2x+7 + 3 \cot 3x - \frac{1}{2x}$$

(i)  $\frac{d}{dx} \log_a x$

$$= \frac{d}{dx} \left( \frac{\ln x}{\ln a} \right)$$

$$= \frac{1}{\ln a} \left( \frac{d}{dx} \ln x \right)$$

$$= \frac{1}{x \ln a}$$

(j)  $\frac{d}{dx} \tan^{-1}(\cos x)$

$$= \frac{1}{1+\cos^2 x} (-\sin x)$$

$$= \frac{-\sin x}{1+\cos^2 x}$$

2. (a)  $e^{\sin x} + xy = y^3 + \sec x$

Differentiating both sides:

$$e^{\sin x} \cos x + y + x \frac{dy}{dx} = 3y^2 \frac{dy}{dx} + \sec x \tan x$$

$$e^{\sin x} \cos x + y - \sec x \tan x = (3y^2 - x) \frac{dy}{dx}$$

$$\frac{dy}{dx} = \frac{e^{\sin x} \cos x + y - \sec x \tan x}{3y^2 - x}$$

(b)  $y = 3^x$

$$\ln y = \ln 3^x = x \ln 3$$

Differentiating both sides:

$$\frac{1}{y} \left( \frac{dy}{dx} \right) = \ln 3$$

$$\frac{dy}{dx} = y \ln 3 = 3^x \ln 3$$

## Part 1 (cont.)

$$\begin{aligned} 2. (c) \quad y &= x^x \\ (\text{cont}) \quad &= e^{\ln(x^x)} \\ &= e^{x \ln x} \end{aligned}$$

$$\begin{aligned} \frac{dy}{dx} &= e^{x \ln x} \left( \frac{d}{dx} x \ln x \right) \\ &= e^{x \ln x} (1 + \ln x) \\ &= x^x (1 + \ln x) \end{aligned}$$

$$\begin{aligned} (d) \quad y &= (\sin x)(\sin^{-1} x)(e^x)(x^2) \\ &= uv \quad (\text{where } u = (\sin x)(\sin^{-1} x); \quad v = (e^x)(x^2)) \rightarrow \text{for simplicity.} \end{aligned}$$

$$\begin{aligned} \frac{du}{dx} &= \sin x \left( \frac{1}{\sqrt{1-x^2}} \right) + \sin^{-1} x (\cos x) \\ &= \frac{\sin x}{\sqrt{1-x^2}} + \cos x \sin^{-1} x \end{aligned}$$

$$\frac{dv}{dx} = e^x (2x) + e^x (x^2) = e^x (x^2 + 2x)$$

$$\frac{dy}{dx} = \frac{du}{dx}(v) + \frac{dv}{dx}(u)$$

$$\begin{aligned} &= \left( \frac{\sin x}{\sqrt{1-x^2}} + \cos x \sin^{-1} x \right) (e^x)(x^2) + [e^x(x^2 + 2x)] (\sin x)(\sin^{-1} x) \\ &= (\sin x)(\sin^{-1} x)(e^x)(x^2) \left( \frac{1}{\sin^{-1} x \sqrt{1-x^2}} + \cot x + 1 + \frac{2}{x} \right) \end{aligned}$$

## Part 2

$$3. (a) \int (x^2 + 1)^3 dx$$

$$= \int (x^4 + 2x^2 + 1)(x^2 + 1) dx$$

$$= \int (x^6 + 2x^4 + x^2 + x^4 + 2x^2 + 1) dx$$

$$= \int (x^6 + 3x^4 + 3x^2 + 1) dx$$

$$= \frac{x^7}{7} + \frac{3x^5}{5} + x^3 + x + C, \text{ where } C \text{ is an arbitrary integer}$$

$$(b) \int \frac{x^3 - 2x + 1}{x^2} dx$$

$$= \int \left( x - \frac{2}{x} + x^{-2} \right) dx$$

$$= \frac{x^2}{2} - 2 \ln|x| - \frac{1}{x} + C, \text{ where } C \text{ is an arbitrary integer}$$

$$\begin{array}{r} (c) \quad x^2 + 4x + 3 \overline{) x^3 + 0x^2 + 0x + 0} \\ \underline{-(x^3 + 4x^2 + 3x)} \phantom{0} \\ -4x^2 - 3x + 0 \\ \underline{-(-4x^2 - 16x - 12)} \\ 13x + 12 \end{array}$$

$$\text{Hence, } x^3 = (x^2 + 4x + 3)(x - 4) + 13x + 12.$$

→ answer continues

## Part 2 (cont.)

3. (c)  $\int \frac{x^2}{x^2+4x+3} dx$   
 (cont.)  $\rightarrow$   
 $= \int (x-4 + \frac{13x+12}{x^2+4x+3}) dx$   
 $= \int (x-4) dx + \int \frac{13x+12}{(x+1)(x+3)} dx$

Let  $\frac{13x+12}{(x+1)(x+3)} = \frac{A}{x+1} + \frac{B}{x+3}$

$Ax+3A+Bx+B = 13x+12$

$A+B=13$

$3A+B=12$

By comparing coefficients,

$A = -\frac{1}{2}; B = \frac{27}{2}$

$= \int (x-4) dx + \int \left[ \frac{1}{2(x+1)} + \frac{27}{2(x+3)} \right] dx$

$= \frac{x^2}{2} - 4x - \frac{1}{2} \ln|x+1| + \frac{27}{2} \ln|x+3| + C$ , where  $C$  is an arbitrary constant

(d)  $\int \frac{x^2-1}{x^3-3x-1} dx$

$= \frac{1}{3} \int \frac{3x^2-3}{x^3-3x-1} dx$

$= \frac{1}{3} \ln|x^3-3x-1| + C$ , where  $C$  is an arbitrary constant

(e)  $\int \frac{1}{x^2+4x+4} dx$

$= \int \frac{1}{(x+2)^2} dx$

$= -\frac{1}{x+2} + C$ , where  $C$  is an arbitrary constant

(f)  $\int \frac{1}{x^2+4x+13} dx$

$= \int \frac{1}{(x+2)^2+3^2} dx$

$= \frac{1}{3} \tan^{-1}\left(\frac{x+2}{3}\right) + C$ , where  $C$  is an arbitrary constant

(g)  $\int \frac{x+4}{x^2+4x+13} dx$

$= \int \frac{x+2}{x^2+4x+13} dx - \int \frac{2}{x^2+4x+13} dx$  from (f)

$= \frac{1}{2} \ln|x^2+4x+13| - \frac{2}{3} \tan^{-1}\left(\frac{x+2}{3}\right) + C$ , where  $C$  is an arbitrary constant

(h)  $\int \frac{1}{\sqrt{15+2x-x^2}} dx$

$= \int \frac{1}{\sqrt{4^2-(x-1)^2}} dx$

$= \sin^{-1}\left(\frac{x-1}{4}\right) + C$ , where  $C$  is an arbitrary constant

(i)  $\int \frac{x}{\sqrt{1-x^2}} dx$  is the integral. Let  $u = \sqrt{1-x^2}$ , then  $\frac{du}{dx} = \frac{-2x}{2\sqrt{1-x^2}} = -\frac{x}{\sqrt{1-x^2}}$

$= \int -\frac{du}{u}$

$= \int -1 du$

$= -u + C$

$= -\sqrt{1-x^2} + C$ , where  $C$  is an arbitrary constant



## Part 2 (cont.)

3. (j)  $\int \frac{x}{\sqrt{15+2x-x^2}} dx$   
(cont.)

$$= \int \frac{x}{\sqrt{16-(x-1)^2}} dx \rightarrow \text{let } u = x-1, \text{ then } \frac{du}{dx} = 1 \text{ and } x = u+1$$

$$= \int \frac{u+1}{\sqrt{16-u^2}} du$$

$$= \int \frac{u}{\sqrt{16-u^2}} du + \int \frac{1}{\sqrt{16-u^2}} du \rightarrow \text{let } v = 16-u^2, \text{ then } \frac{dv}{du} = -2u, u = -\frac{1}{2} \left( \frac{dv}{du} \right)$$

$$= \int \frac{-\frac{1}{2} \left( \frac{dv}{du} \right)}{\sqrt{v}} du + \int \frac{1}{\sqrt{16-u^2}} du$$

$$= \int -\frac{1}{2\sqrt{v}} dv + \int \frac{1}{\sqrt{16-u^2}} du$$

$$= -\sqrt{v} + \sin^{-1} \left( \frac{u}{4} \right) + C$$

$$= -\sqrt{16-u^2} + \sin^{-1} \left( \frac{x-1}{4} \right) + C$$

$$= -\sqrt{16-(x-1)^2} + \sin^{-1} \left( \frac{x-1}{4} \right) + C$$

$$= -\sqrt{15+2x-x^2} + \sin^{-1} \left( \frac{x-1}{4} \right) + C, \text{ where } C \text{ is an arbitrary constant}$$

4. (a)  $\int \sec^2(4x) dx$

$$= \frac{\tan(4x)}{4} + C, \text{ where } C \text{ is an arbitrary constant}$$

(b)  $\int \tan^2 x dx$

$$= \int (\sec^2 x - 1) dx$$

$$= \tan x - x + C, \text{ where } C \text{ is an arbitrary constant}$$

(c)  $\int \tan 2x dx$

$$= \int \frac{\sin 2x}{\cos 2x} dx$$

$$= \int \frac{-2 \sin 2x}{\cos 2x} dx$$

$$= -\frac{1}{2} \ln |\cos 2x| + C, \text{ where } C \text{ is an arbitrary constant}$$

(d)  $\int \frac{4 \sin x}{1 - \cos x} dx$

$$= 4 \int \frac{\sin x}{1 - \cos x} dx$$

$$= 4 \ln |1 - \cos x| + C, \text{ where } C \text{ is an arbitrary constant}$$

(e)  $\int \sin 3x \sin 2x dx$

$$= -\frac{1}{2} \int (\cos 5x - \cos x) dx$$

$$= -\frac{1}{2} \left( \frac{\sin 5x}{5} - \sin x \right) + C$$

$$= \frac{5 \sin x - \sin 5x}{10} + C, \text{ where } C \text{ is an arbitrary constant}$$

## Part 2 (cont.)

4. (f)  $\int_0^{\frac{\pi}{4}} \sec^4 x \, dx$

$$= \int_0^{\frac{\pi}{4}} (\sec^2 x)(\sec^2 x) \, dx$$

$$= \int_0^{\frac{\pi}{4}} (1 + \tan^2 x)(\sec^2 x) \, dx$$

→ let  $u = \tan x$ ,  $\frac{du}{dx} = \sec^2 x$ ; the lower bound remains 0 and upper bound becomes  $\tan \frac{\pi}{4} = 1$ .

$$= \int_0^1 (1 + u^2) \, du$$

$$= \left[ u + \frac{u^3}{3} \right]_0^1$$

$$= \left[ \tan x + \frac{\tan^3 x}{3} \right]_0^1$$

$$= 1 + \frac{1}{3}$$

$$= \frac{4}{3}$$

5. (a)  $\int (e^{2-x} + e^{3x-5} + 2^x + e) \, dx$

$$= \int e^{2-x} \, dx + \int e^{3x-5} \, dx + \int 2^x \, dx + \int e \, dx$$

$$= -e^{2-x} + \frac{e^{3x-5}}{3} + \frac{2^x}{\ln 2} + ex + C, \text{ where } C \text{ is an arbitrary constant}$$

(b)  $\int \frac{1}{1+e^x} \, dx$

$$= \int \frac{1+e^x - e^x}{1+e^x} \, dx$$

$$= \int 1 \, dx - \int \frac{e^x}{1+e^x} \, dx \quad \rightarrow \text{let } u = 1+e^x, \frac{du}{dx} = e^x, du = e^x dx$$

$$= \int 1 \, dx - \int \frac{1}{u} \, du$$

$$= x - \ln|u| + C$$

$$= x - \ln(1+e^x) + C, \text{ where } C \text{ is an arbitrary constant}$$

(c)  $\int_0^2 x e^{x^2} \, dx \quad \rightarrow \text{let } u = x^2, \frac{du}{dx} = 2x, \text{ upper bound changes to } 4$

$$= \int_0^4 \frac{1}{2} \left( \frac{du}{dx} \right) e^u \, dx$$

$$= \frac{1}{2} \int_0^4 e^u \, du$$

$$= \frac{1}{2} [e^u]_0^4$$

$$= \frac{1}{2}(e^4 - 1)$$

## Part 2 (cont.)

5. (d)  $\int x e^x dx \rightarrow \text{let } u = x, du = dx, \frac{dv}{dx} = e^x, v = e^x$   
(cont.)  
 $= x e^x - \int e^x dx$   
 $= e^x (x-1) + C$ , where  $C$  is an arbitrary constant.

6. (a)  $\int x \ln x dx \rightarrow \text{let } u = \ln x, du = \frac{1}{x} dx, \frac{dv}{dx} = 1, v = x$ .  
 $= x \ln x - \int x \left(\frac{1}{x} dx\right)$   
 $= x \ln x - x + C$ , where  $C$  is an arbitrary constant.

(b)  $\int \tan^{-1} x dx \rightarrow \text{let } u = \tan^{-1} x, \frac{du}{dx} = \frac{1}{1+x^2}, \frac{dv}{dx} = 1, v = x$ .  
 $= x \tan^{-1} x - \int x \left(\frac{1}{1+x^2}\right) dx$   
 $= x \tan^{-1} x - \frac{1}{2} \int \frac{2x}{1+x^2} dx$   
 $= x \tan^{-1} x - \frac{1}{2} \ln(1+x^2) + C$ , where  $C$  is an arbitrary constant.

## Part 3

1. (i) Differentiating the equation of the curve on both sides:

$$4x - 3 \left( x \frac{dy}{dx} + y \right) + 2y \frac{dy}{dx} = 0$$

$$4x - 3y = (3x - 2y) \frac{dy}{dx}$$

$$\frac{dy}{dx} = \frac{4x - 3y}{3x - 2y}$$

At the point  $(4, 3)$ ,  $x=4$  and  $y=3$ , hence

$$\frac{dy}{dx} = \frac{4(4) - 3(3)}{3(4) - 2(3)} = \frac{7}{6}$$

$$y = \frac{7}{6}x + C \rightarrow C = 3 - \frac{7}{6}(4) = -\frac{5}{3}$$

$$\text{Eqn. of tangent is } y = \frac{7}{6}x - \frac{5}{3} \rightarrow 6y = 7x - 10$$

(ii)  $m_{\text{normal}} = -\frac{1}{m_{\text{tangent}}} = -\frac{6}{7}$

$$y = -\frac{6}{7}x + C \rightarrow C = 3 + \frac{6}{7}(4) = \frac{45}{7}$$

$$\text{Eqn. of normal is } y = -\frac{6}{7}x + \frac{45}{7} \rightarrow 7y = -6x + 45$$

2. (i)  $\frac{dy}{dx} = \frac{1}{2\sqrt{x}}$

$$\left. \frac{dy}{dx} \right|_{x=16} = \frac{1}{2\sqrt{16}} = \frac{1}{8}$$

$$\text{At } (16, 4), y = \frac{1}{8}x + C \rightarrow C = 4 - \frac{16}{8} = 2$$

$$\text{Eqn. of tangent is } y = \frac{1}{8}x + 2 \rightarrow 8y = x + 16$$

### Part 3 (cont.)

2. (i) When  $x = 16.01$ ,  
(cont.)

$$\begin{aligned} y &\approx y|_{x=16} + \left(\frac{dy}{dx}\right)|_{x=16} (16.01 - 16) \\ &= 4 + \frac{1}{8} (0.01) \\ &= 4.00125 \end{aligned}$$

$$(ii) \frac{d^2y}{dx^2} = \frac{d}{dx} \left( \frac{1}{2} x^{-\frac{1}{2}} \right) = -\frac{1}{4} x^{-\frac{3}{2}}$$

$$\left. \frac{d^2y}{dx^2} \right|_{x=16} = -\frac{1}{4} \left( \frac{16^{\frac{3}{2}}}{16} \right) = -\frac{1}{4} \left( \frac{64}{16} \right) = -\frac{1}{16} < 0$$

So at  $(16, 4)$ , the curve is concave down.

Hence the linear approximation is an overestimate.

$$\begin{aligned} 3. (i) f'(x) &= \frac{(cx+d)(a) - (ax+b)(c)}{(cx+d)^2} \\ &= \frac{acx+ad-acx-bc}{(cx+d)^2} \\ &= \frac{ad-bc}{(cx+d)^2} \end{aligned}$$

If  $ad-bc \neq 0$ , then  $f'(x) \neq 0$ .

Hence the graph of  $y=f(x)$  has no stationary points.

$$(ii) \text{ From (i), } f'(x) = \frac{3(1) - (-7)(2)}{(2x+1)^2} = \frac{17}{(2x+1)^2} > 0, \quad x \neq -\frac{1}{2}.$$

Hence as  $f'(x)$  is always positive on all points other than  $x = -\frac{1}{2}$  (where it is undefined), the graph of  $y$  is increasing (for any interval on the graph that does not contain  $x = -\frac{1}{2}$ ).

$$(iii) \lim_{x \rightarrow \infty} \frac{3x-7}{2x+1}$$

$$= \lim_{x \rightarrow \infty} \frac{3 - \frac{7}{x}}{2 + \frac{1}{x}}$$

$$= \frac{3}{2} \quad (\text{the horizontal asymptote is thus } y = \frac{3}{2}).$$

From (ii), the vertical asymptote is  $x = -\frac{1}{2}$ .

$$4. \text{ We have } \frac{dV}{dt} = -2 \text{ cm}^3/\text{s}.$$

$$V = \frac{1}{3} \pi r^2 h = \frac{1}{3} \pi \left( \frac{h}{3} \right)^2 h = \frac{1}{27} \pi h^3 \quad (r = \frac{h}{3} \text{ by similar triangles})$$

$$\frac{dV}{dh} = \frac{1}{9} \pi h^2$$

$$\frac{dh}{dt} = \frac{dV}{dt} \div \frac{dV}{dh}$$

$$\left. \frac{dh}{dt} \right|_{h=6} = -2 \div \frac{1}{9} \pi (6^2) = -\frac{1}{2} \pi \text{ cm/s}$$



Part 3 (cont.)

5. We have  $x^2 + y^2 = r^2 = 25 \text{ cm}^2$  so  $y = \sqrt{25 - x^2}$

$$A = 2xy = 2x\sqrt{25 - x^2}$$

$$\frac{dA}{dx} = 2 \left[ x \frac{d}{dx} \sqrt{25 - x^2} + \sqrt{25 - x^2} \left( \frac{d}{dx} x \right) \right]$$

$$= 2 \left[ x(-2x) \left( \frac{1}{2\sqrt{25 - x^2}} \right) + \sqrt{25 - x^2} \right]$$

$$= 2 \left( \frac{-x^2}{\sqrt{25 - x^2}} + \frac{25 - x^2}{\sqrt{25 - x^2}} \right)$$

$$= \frac{50 - 4x^2}{\sqrt{25 - x^2}}$$

To find stationary points, we set  $\frac{dA}{dx} = 0$ , i.e.

$$50 - 4x^2 = 0, \text{ hence } x^2 = \frac{25}{2} \text{ and } x = \frac{5}{\sqrt{2}}.$$

$$A = 2x\sqrt{25 - x^2} = 2 \left( \frac{5}{\sqrt{2}} \right) \sqrt{25 - \frac{25}{2}} = 5(\sqrt{2}) \left( \sqrt{\frac{25}{2}} \right) = 25 \text{ cm}^2$$